TFTP_Proofs.v
@@ -1,0 +1,47 @@
+Require Import ZArith.
+Require Import Coq.Strings.String.
+Require Import ZArith.BinInt.
+Require Import Ascii.
+Require Import List.
+Require String.
+Require Import Coq.Numbers.Natural.Abstract.NDiv.
+
+(* Require Import Binding. *)
+Set Implicit Arguments.
+
+Import ListNotations.
+
+Local Open Scope char_scope.
+Local Open Scope N_scope.
+
+Require Import TFTP_Core.
+
+Search "Serialize".
+Theorem N_2b_correctness1 : forall x:N, (x < 256*256) -> Get2bN (Nto2b x) = Some x.
+  intros.
+  unfold N_to_2b, get_2b_N.
+  f_equal.
+  assert (N_of_ascii
+            (ascii_of_N (x / 256)) = x / 256).
+  * apply N_ascii_embedding.
+    assert (256 * (x/256) <= x).
+    ** eapply N.mul_div_le. zify; omega.
+    ** zify; omega.
+  * assert (N_of_ascii (ascii_of_N (x mod 256)) = x mod 256).
+    ** apply N_ascii_embedding. apply N.mod_upper_bound. zify; omega.
+    ** assert (x mod 256 = x - 256 * (x / 256)).
+       *** apply N.mod_eq. zify; omega.
+       *** rewrite -> H0. rewrite -> H1.
+           rewrite -> H2.
+           remember (256 * (x / 256)) as M.
+           assert (M <= x).
+           **** rewrite -> HeqM. apply N.mul_div_le. zify; omega.
+           **** zify; omega.
+Qed.
+
+Theorem SerializationCorrectness : forall m : TFTPMessage, Deserialize (Serialize m) = Some m.
+  intros.
+  unfold Serialize.
+  unfold Deserialize.
+  admit.
+Admitted. (* TODO *)
